<?xml version="1.0"?>


<!DOCTYPE rdf:RDF [
    <!ENTITY rules "http://rules#" >
    <!ENTITY owl "http://www.w3.org/2002/07/owl#" >
    <!ENTITY xsd "http://www.w3.org/2001/XMLSchema#" >
    <!ENTITY rdfs "http://www.w3.org/2000/01/rdf-schema#" >
    <!ENTITY rdf "http://www.w3.org/1999/02/22-rdf-syntax-ns#" >
]>


<rdf:RDF xmlns="http://rules#"
     xml:base="http://rules"
     xmlns:rules="http://rules#"
     xmlns:xsd="http://www.w3.org/2001/XMLSchema#"
     xmlns:rdfs="http://www.w3.org/2000/01/rdf-schema#"
     xmlns:rdf="http://www.w3.org/1999/02/22-rdf-syntax-ns#"
     xmlns:owl="http://www.w3.org/2002/07/owl#">
    <owl:Ontology rdf:about="http://rules#">
        <owl:versionIRI rdf:resource="http://rules/v.2"/>
    </owl:Ontology>
    


    <!-- 
    ///////////////////////////////////////////////////////////////////////////////////////
    //
    // Annotation properties
    //
    ///////////////////////////////////////////////////////////////////////////////////////
     -->

    


    <!-- 
    ///////////////////////////////////////////////////////////////////////////////////////
    //
    // Datatypes
    //
    ///////////////////////////////////////////////////////////////////////////////////////
     -->

    


    <!-- 
    ///////////////////////////////////////////////////////////////////////////////////////
    //
    // Object Properties
    //
    ///////////////////////////////////////////////////////////////////////////////////////
     -->

    


    <!-- http://rules#ContainmentProperty -->

    <owl:ObjectProperty rdf:about="&rules;ContainmentProperty">
        <rdfs:label>Containment property</rdfs:label>
        <rdfs:comment>Used as the super proeprty of properties which mean containment relation between resources. Super property is rdfs:subPropertyOf.</rdfs:comment>
        <rdfs:subPropertyOf rdf:resource="&rules;rules"/>
    </owl:ObjectProperty>
    


    <!-- http://rules#RelationProperty -->

    <owl:ObjectProperty rdf:about="&rules;RelationProperty">
        <rdfs:label>Relational (referential) property</rdfs:label>
        <rdfs:comment>Used as the super proeprty of properties which mean relation (references) between resources. Super property is rdfs:subPropertyOf.</rdfs:comment>
        <rdfs:subPropertyOf rdf:resource="&rules;rules"/>
    </owl:ObjectProperty>
    


    <!-- http://rules#rules -->

    <owl:ObjectProperty rdf:about="&rules;rules"/>
    


    <!-- 
    ///////////////////////////////////////////////////////////////////////////////////////
    //
    // Classes
    //
    ///////////////////////////////////////////////////////////////////////////////////////
     -->

    


    <!-- http://rules#RootElement -->

    <owl:Class rdf:about="&rules;RootElement">
        <rdfs:label>Root Element</rdfs:label>
        <rdfs:comment>Superclass of elements which are roots of a heirarchical structure</rdfs:comment>
    </owl:Class>
</rdf:RDF>



<!-- Generated by the OWL API (version 3.2.3.1824) http://owlapi.sourceforge.net -->

